\documentclass[a4paper]{article}
\input{../../preamble.tex}
\title{какой то семинар}
\begin{document}
\maketitle
	\[
	H =L_2 \left( \left[ 0,1 \right] \times [0,1] \right) 
.\] 
\[
	A= \frac{\partial ^2}{\partial x^2} + i \frac{\partial }{\partial y} 
.\] 
\[
	D(A)= \left\{  u \in  H : u'_x \mid _{x=0}=u \mid _{x=1}=0, \; u \mid _{y=0}=-u \mid _{y=1} \right\} 
.\] 
\begin{problem}
	\begin{enumerate}
		\item Д-ть, что $A$ -- сим.
		\item Найти  в $H$ ортогон. базис из с. ф. $A$ 
		\item Найти обл. опр. и спектр. разл. $\overline{A}$ 
		\item Решение задачи
			\[
				\frac{d}{dt}u(t) +\left(\overline{A}\right)^2 u= e^{it}, \quad t >0 ,\quad u(t) \in D\left(\overline{A}^2\right)
			\]
			\[
				u(+0)=0
			.\] 
	\end{enumerate}
\end{problem}

\begin{sol}
\begin{enumerate}
\item
	$u,\,v \in D(A)$ 
	\[
		\left( Au,\,v \right) \textover{=}{?} (u,\,Av)
	.\] 
\begin{multline*}
	\left( Av,\,u \right) = \int\limits_{0}^{1} \int\limits_{0}^{1}  (u_{x x} + i u_{y}) \overline{v} dx dy= \int\limits_{0}^{1} 
	dy \int\limits_{0}^{1} u_{x x} \overline{v}dx+i
	\int\limits_{0}^{1} dx \int\limits_{0}^{1}  u_y \overline{v} dy =\\= \int\limits_{0}^{1} dy \left( 
	\underbrace{u_x \overline{v}\mid _{0}^1}_{u_{x}\mid _{x=1}
\cdot \underbrace{\overline{v}\mid _{x=1}}_{=0}-\underbrace{u_x \mid _{x=0}\cdot \overline{v}\mid _{x=0}}_{}}\right)   
\ldots\end{multline*} 
\begin{enumerate}
	\item $L_2 \left( [0,1] \times [0,1] \right) =
		L_2 [0,1] \otimes L_2[0,1], \; \otimes$ --- это $\cdot$ 
	\item $H_1\otimes H_2$, $\{f_n\} $ --- ортог. базис в
		$H_1$, $\{g_n\} $ --- ортог. базис в $H_2$ 
		$\implies$ $\{f_n \otimes g_m\} $ --- ортог. базис в 
		$H_1 \otimes H_2$
\end{enumerate}
\item
\begin{enumerate}
	\item $f_(x)$ т.ч. $f'' =\lambda f,\; f'(0)=0, f(1)=0$
 \begin{enumerate}
	\item $\lambda> 0$ 
		\[
		f=
		A \sh \sqrt{\lambda} x +B \ch \sqrt{\lambda}  x
		\]
			\[
			\begin{aligned}
			f'(0) = A \sqrt{\lambda} =0 \to  A=0\\ f(1)= B \ch \sqrt{\lambda} \to B=0
			\end{aligned} \to \emptyset
		.\] 
	\item  $\lambda=0$
		 \[
		f=\underbrace{Ax}_{=0}+B
		.\]
		\[
			\begin{aligned}
			f'(0)=A=0
			f(1)=B=0	
			\end{aligned}\implies \emptyset
		.\] 
	\item $\lambda<0$ 
		\[
		f= A \underbrace{\sin \sqrt{-\lambda} x}_{=0}+
		B \cos \sqrt{-\lambda} x
		.\] 
		\[
			f'(0) = A \sqrt{ -\lambda} =0,\, A=0
		.\] 
		\[
			f(1)=B \cos \sqrt{-\lambda} =0 \implies
			\cos \sqrt{-\lambda} =0 \implies
			\sqrt{-\lambda} = \frac{\pi}{2} +\pi n
		.\] 
		\[
			\lambda_n = -\left( \frac{\pi}{2}+\pi n \right) ^2
		.\] 
		\[
			f_n = \cos \left( \frac{\pi}{2}+\pi n \right) x
		.\] 
\end{enumerate}
\item   $g(y)$ т.ч. $i g' = \mu g$, $g(0)=-g (1)$ 
	\[
	g'=-i \mu g
	.\] 
	\[
	g = A e ^{-i \mu g}
	.\] 
	\[
		g(0) =A = -g(1) = -A e ^{-i\mu}
	.\] 
	\[
	1= -e ^{i\mu}
	.\] 
	\[
	e^{-i\mu}= -1 = e ^{i \pi +2 \pi m i}
	.\] 
	\[
	-i \mu = i \pi +2 \pi m i
	.\] 
	\[
	\mu_m = - \pi - 2 \pi m
	.\] 
	\[
		g_m= e ^{\left( \pi +2 \pi m  \right) iy}
	.\] 
	\[
		e_{n,\,m}= \cos \left( \frac{\pi}{2} +\pi n \right)
		x \cdot e^{(\pi +2 \pi m) i y}
	.\] 
	\[
		\lambda_{n,\,m}= -\left( \frac{\pi}{2}+\pi n \right) ^2 - \left( \pi +2 \pi m \right) 
	.\] 
	\[
	\sqrt{-\lambda_n} = \frac{\pi}{2}+ \pi n
	.\] 
\end{enumerate}
\item  
	\[
		\overline{A} = \sum_{n=0}^{\infty} \sum_{m=-\infty}^{+\infty}  \lambda_{n,\,m} \frac{(u,\, e_{n,\,m})}{(e_{n,\,m},\,
		e_{n,\,m}}e_{n,\,m} \leftarrow \text{спектр. разл}
	.\] 
	\[
		D\left(\overline{A}\right) =
		\left\{ u \in L_2 \left( [0,\,1]\times [0,\,1] \right): \sum_{n=0}^{\infty} \sum_{m=-\infty}^{+\infty} \lambda_{n,\,m}^2
		\frac{\left| \left( u,\,e_{n,\,m} \right)  \right| ^2}{\| e_{n,\,m}\|^2}<\infty\right\} 
	.\] 
\item 
\[
	u = \sum_{n,\,m}^{\infty} T_{n,\,m}(t) e_{n,\,m}; \;
	\overline{A}^2 u = \sum_{n,\,m}^{} \lambda_{n,\,m}^2
	T_{n,\,m} e_{n,\,m}
.\] 
\begin{multline*}
1= \sum_{n,\, m}^{} \alpha_{n,\,m} e_{n,\,m}, \; \alpha_{n,\,m}
= \frac{\left( 1,\, e_{n,\,m} \right) }{\left( e_{n,\,m},
e_{n,\,m}\right) }=\\=
\frac{\int\limits_{0}^{1} \int\limits_{0}^{1}  \cos
\left( \frac{\pi}{2} +\pi n \right) x \cdot e ^{-i (\pi+2
\pi m) y}dx dy}{\int\limits_{0}^{1}  \cos^2 \left( \frac{\pi}{2}
+\pi n\right) x dx \int\limits_{0}^{1}  e ^{i \left( \pi
+2m \pi\right) y} e^{-i(\pi+2\pi m)y}dy
 }=\\=\sum_{n,\,m}^{} T_{n,\,m}' e_{n,\,m}+ \sum_{n,\,m}^{} \lambda^2_{n,\,m}T_{n,\,m} e_{n,\,m} = \sum_{n,\,m}^{} \alpha_{n,\,m}e_{n,\,m}
 \cdot e^{it}.\end{multline*} 
 \[
\left\{
\begin{aligned}
	T_{n,\,m}'+\lambda_{n,\,m}^2 T_{n,\,m}&=\alpha_{n,\,m}e^{it}\\
	T_{n,\,m}(0)&=0
\end{aligned}
\right.
 \] 
\[
T_{n,\,m}= C_{n,\,m} e ^{-\lambda^2_{n,\,m} t}+ \beta_{n,\,m}e^{it}
.\] 
\[
\beta_{n,\,m }\ldots
\]
\[
	u(t,\,x,\,y)= \sum_{n,\,m}^{} \frac{\alpha_{n,\,m}}{i +\lambda_{n,\,m}^2}\left[ -e ^{- \lambda_{n,\,m}^2 t}+e^{it} \right] e_{n,\,m}
.\] 
\emph{Проверки}
\[
	u \in  L_2 [0,\,1]\times [0,\,1])
.\] 
\begin{multline*}
|u|^2= \sum_{n,\,m}^{} \frac{|\alpha_{n,\,m}|^2}{|i+\lambda_{n,\,m}^2|^2}\left| -e ^{- \lambda_{n,\,m}^2 t}+ e ^{it} \right| ^2 \| e_{n,\,m}\|^2 \le  \sum_{n,\,m}^{} \frac{|\alpha_{n,\,m}|^2}{1+\lambda_{,\,m}^4}\cdot 4 \| e_{n,\,m}\|<\\<\ldots< +\infty
.\end{multline*} 
\end{enumerate}
\end{sol}

\end{document}
